src/Init/Data/Nat/Lemmas.lean
@@ -578,7 +578,7 @@ theorem mul_eq_zero : ∀ {m n}, n * m = 0 ↔ n = 0 ∨ m = 0
   | _, 0 => ⟨fun _ => .inl rfl, fun _ => Nat.zero_mul ..⟩
   | _+1, _+1 => ⟨nofun, nofun⟩
 
-protected theorem mul_ne_zero_iff : n * m ≠ 0 ↔ n ≠ 0 ∧ m ≠ 0 := by rw [ne_eq, mul_eq_zero, not_or]
+protected theorem mul_ne_zero_iff : n * m ≠ 0 ↔ n ≠ 0 ∧ m ≠ 0 := by rw [mul_eq_zero, not_or]
 
 protected theorem mul_ne_zero : n ≠ 0 → m ≠ 0 → n * m ≠ 0 := (Nat.mul_ne_zero_iff.2 ⟨·,·⟩)
 
